updated main theorem

src/proofs/no_slashable_blocks/supporting_lemmas/ind_inv_implies_safety/ind_inv_implies_safety.dfy
@@ -1,70 +1,43 @@
-include "../../../../common/commons.dfy"
-include "../../common/attestation_creation_instrumented.dfy"
-include "../../../../specs/consensus/consensus.dfy"
-include "../../../../specs/network/network.dfy"
-include "../../../../specs/dv/dv_attestation_creation.dfy"
-include "../../../../specs/dvc/dvc_attestation_creation.dfy"
+include "../../../../common/block_proposer/block_types.dfy"
+include "../../../../common/block_proposer/block_common_functions.dfy"
+include "../../../../common/block_proposer/block_signing_functions.dfy"
+include "../../common/dvc_block_proposer_instrumented.dfy"
 
-include "../../../common/helper_sets_lemmas.dfy"
-include "../../../no_slashable_attestations/common/common_proofs.dfy"
-include "../../../no_slashable_attestations/common/dvc_spec_axioms.dfy"
-
-include "../dv_next_preserves_ind_inv/proofs_intermediate_steps.dfy"
-include "../dv_next_preserves_ind_inv/ind_inv_dv_next.dfy"
+include "../../../../specs/consensus/block_consensus.dfy"
+include "../../../../specs/network/block_network.dfy"
+include "../../../../specs/dv/dv_block_proposer.dfy"
 
 include "../inv.dfy"
 include "../ind_inv.dfy"
-
-include "core_proofs.dfy"
+// include "../dv_next_preserves_ind_inv/proofs_intermediate_steps.dfy"
 
 
 module Ind_Inv_Implies_Safety
 {
-    import opened Types 
-    import opened CommonFunctions
-    import opened ConsensusSpec
-    import opened NetworkSpec
-    import opened DVC_Spec
-    import opened DV
-    import opened Att_Ind_Inv_With_Empty_Init_Att_Slashing_DB
-    import opened Att_Inv_With_Empty_Initial_Attestation_Slashing_DB
-    
-    import opened Core_Proofs
-    import opened Ind_Inv_DV_Next
-    import opened Proofs_Intermediate_Steps 
+    import opened Block_Types
+    import opened Block_Signing_Functions
+    import opened Block_Common_Functions
+    import opened Block_Consensus_Spec
+    import opened Block_Network_Spec
+    import opened DVC_Block_Proposer_Spec_Instr
+    import opened DV_Block_Proposer_Spec 
+    import opened Block_Inv_With_Empty_Initial_Block_Slashing_DB
+    import opened Block_Ind_Inv_With_Empty_Initial_Block_Slashing_DB
+    // import opened Proofs_Intermediate_Steps
 
-    predicate non_slashable_attestations(
+    predicate non_slashable_submitted_blocks(
         dv: DVState
     )
     {
-        forall a: Attestation, a': Attestation
-                | 
-                && a in dv.all_attestations_created
-                && is_valid_attestation(a, dv.dv_pubkey)
-                && a' in dv.all_attestations_created
-                && is_valid_attestation(a', dv.dv_pubkey)     
-                ::
-                && !is_slashable_attestation_data_eth_spec(a.data, a'.data)
-                && !is_slashable_attestation_data_eth_spec(a'.data, a.data)
+        && inv_slots_in_slashing_db_is_not_higher_than_slot_of_latest_proposer_duty(dv)
+        && inv_at_most_submitted_signed_beacon_block_for_every_slot(dv)
     }
 
-    lemma lem_ind_inv_no_slashable_submitted_attestations(dv: DVState)
+    lemma lem_ind_inv_no_slashable_submitted_blocks(dv: DVState)
     requires ind_inv(dv)    
-    ensures non_slashable_attestations(dv)
+    ensures non_slashable_submitted_blocks(dv)
     {   
-        lem_ind_inv_implies_intermediate_steps(dv);
-
-        forall a: Attestation, a': Attestation
-                    | 
-                    && a in dv.all_attestations_created
-                    && is_valid_attestation(a, dv.dv_pubkey)
-                    && a' in dv.all_attestations_created
-                    && is_valid_attestation(a', dv.dv_pubkey)     
-        ensures && !is_slashable_attestation_data_eth_spec(a.data, a'.data)
-                && !is_slashable_attestation_data_eth_spec(a'.data, a.data);
-        {
-            lem_no_slashable_submitted_attestations(dv, a, a');
-        }
+        // lem_ind_inv_implies_intermediate_steps(dv);
     }
 
 }
