src/proofs/no_slashable_blocks/main_theorem.dfy
@@ -9,9 +9,9 @@ include "supporting_lemmas/ind_inv_implies_safety/ind_inv_implies_safety.dfy"
 
 module No_Slashable_Attestations_Main_Theorem
 {
-    import opened Types 
-    import opened DV    
-    import opened Att_Ind_Inv_With_Empty_Init_Att_Slashing_DB
+    import opened Block_Types
+    import opened DV_Block_Proposer_Spec    
+    import opened Block_Ind_Inv_With_Empty_Initial_Block_Slashing_DB
     import opened Ind_Inv_DV_Init
     import opened Ind_Inv_DV_Next
     import opened Ind_Inv_Implies_Safety
@@ -21,21 +21,21 @@ module No_Slashable_Attestations_Main_Theorem
         trace: iseq<DVState>
     )  
     {
-        && DV.Init(trace[0], {})
+        && DV_Block_Proposer_Spec.Init(trace[0], {})
         && (
             forall i: Slot ::
-                DV.NextPreCond(trace[i]) ==> DV.Next(trace[i], trace[i+1])
+                DV_Block_Proposer_Spec.NextPreCond(trace[i]) ==> DV_Block_Proposer_Spec.Next(trace[i], trace[i+1])
         )
     }  
 
-    lemma lem_non_slashable_attestations_rec(
+    lemma lem_non_slashable_submitted_blocks_rec(
         trace: iseq<DVState>,
         i: Slot
     )
     requires isValidTrace(trace)
     ensures forall j | 0 <= j <= i ::
-        && NextPreCond(trace[j])  
-        && ind_inv(trace[j])
+                && NextPreCond(trace[j])  
+                && ind_inv(trace[j])
     {
         if i == 0 
         {
@@ -43,23 +43,23 @@ module No_Slashable_Attestations_Main_Theorem
         }
         else 
         {
-            lem_non_slashable_attestations_rec(trace, i-1);
+            lem_non_slashable_submitted_blocks_rec(trace, i-1);
             lem_ind_inv_dv_ind_inv_NextPreCond(trace[i-1], trace[i]);
         }
     }
 
-    lemma lem_non_slashable_attestations(
+    lemma lem_non_slashable_submitted_blocks(
         trace: iseq<DVState>
     )
     requires isValidTrace(trace)
-    ensures forall i:nat :: non_slashable_attestations(trace[i])
+    ensures forall i:nat :: non_slashable_submitted_blocks(trace[i])
     {
         forall i:nat
         ensures ind_inv(trace[i])
-        ensures non_slashable_attestations(trace[i])
+        ensures non_slashable_submitted_blocks(trace[i])
         {
-            lem_non_slashable_attestations_rec(trace, i);
-            lem_ind_inv_no_slashable_submitted_attestations(trace[i]);
+            lem_non_slashable_submitted_blocks_rec(trace, i);
+            lem_ind_inv_no_slashable_submitted_blocks(trace[i]);
         }
         
     }    
