src/proofs/no_slashable_blocks/supporting_lemmas/dv_next_preserves_ind_inv/ind_inv_dv_next.dfy
@@ -1,13 +1,12 @@
-include "../../../../common/commons.dfy"
-include "../../common/attestation_creation_instrumented.dfy"
-include "../../../../specs/consensus/consensus.dfy"
-include "../../../../specs/network/network.dfy"
-include "../../../../specs/dv/dv_attestation_creation.dfy"
-include "../../../../specs/dvc/dvc_attestation_creation.dfy"
+include "../../../../common/block_proposer/block_types.dfy"
+include "../../../../common/block_proposer/block_common_functions.dfy"
+include "../../../../common/block_proposer/block_signing_functions.dfy"
+include "../../common/dvc_block_proposer_instrumented.dfy"
+include "../../common/block_dvc_spec_axioms.dfy"
 
-include "../../../common/helper_sets_lemmas.dfy"
-include "../../../no_slashable_attestations/common/common_proofs.dfy"
-include "../../../no_slashable_attestations/common/dvc_spec_axioms.dfy"
+include "../../../../specs/consensus/block_consensus.dfy"
+include "../../../../specs/network/block_network.dfy"
+include "../../../../specs/dv/dv_block_proposer.dfy"
 
 include "invs_fnc_1.dfy"
 include "invs_fnc_2.dfy"
@@ -24,15 +23,18 @@ include "proofs_intermediate_steps.dfy"
 
 module Ind_Inv_DV_Next
 {
-    import opened Types 
-    import opened CommonFunctions
-    import opened ConsensusSpec
-    import opened NetworkSpec
-    import opened DVC_Spec
-    import opened DV
-    import opened Att_Ind_Inv_With_Empty_Init_Att_Slashing_DB
-    import opened Att_Inv_With_Empty_Initial_Attestation_Slashing_DB
-    import opened Helper_Sets_Lemmas
+    import opened Block_Types
+    import opened Block_Signing_Functions
+    import opened Block_Common_Functions
+    import opened Block_Consensus_Spec
+    import opened Block_Network_Spec
+    import opened DVC_Block_Proposer_Spec_Instr
+    import opened DVC_Block_Proposer_Spec_Axioms
+    import opened Block_Inv_With_Empty_Initial_Block_Slashing_DB
+    import opened Block_Ind_Inv_With_Empty_Initial_Block_Slashing_DB
+    import opened DV_Block_Proposer_Spec    
+    import opened Fnc_Invs_1
+    import opened Fnc_Invs_2
     import opened Invs_DV_Next_1
     import opened Invs_DV_Next_2
     import opened Invs_DV_Next_3
@@ -41,412 +43,425 @@ module Ind_Inv_DV_Next
     import opened Proofs_Intermediate_Steps
     
 
-    lemma lem_ind_inv_dv_next_invs_group_1(dv: DVState, e: DV.Event, dv': DVState)       
-    requires DV.NextEventPreCond(dv, e)
-    requires DV.NextEvent(dv, e, dv')  
+    lemma lem_ind_inv_dv_next_invs_group_1(dv: DVState, e: DV_Block_Proposer_Spec.Event, dv': DVState)       
+    requires DV_Block_Proposer_Spec.NextEventPreCond(dv, e)
+    requires DV_Block_Proposer_Spec.NextEvent(dv, e, dv')  
     requires ind_inv(dv)
     ensures invs_group_1(dv')
     {    
         lem_inv_quorum_constraints_dv_next(dv, e, dv');
         lem_inv_unchanged_paras_of_consensus_instances_dv_next(dv, e, dv');
-        lem_inv_only_dv_construct_signed_attestation_signature_dv_next(dv, e, dv');
-        lem_inv_current_att_duty_is_rcvd_duty_dv_next(dv, e, dv');
+        lem_inv_only_dv_construct_complete_signing_functions_dv_next(dv, e, dv');
+        lem_inv_current_proposer_duty_is_rcvd_duty_dv_next(dv, e, dv');
         lem_inv_latest_served_duty_is_rcvd_duty_dv_next(dv, e, dv');        
     }
 
-    lemma lem_ind_inv_dv_next_invs_group_2(dv: DVState, e: DV.Event, dv': DVState)       
-    requires DV.NextEventPreCond(dv, e)
-    requires DV.NextEvent(dv, e, dv')  
+    lemma lem_ind_inv_dv_next_invs_group_2(dv: DVState, e: DV_Block_Proposer_Spec.Event, dv': DVState)       
+    requires DV_Block_Proposer_Spec.NextEventPreCond(dv, e)
+    requires DV_Block_Proposer_Spec.NextEvent(dv, e, dv')  
     requires ind_inv(dv)
     ensures invs_group_2(dv')
     {
-        lem_inv_none_latest_served_duty_implies_none_current_att_duty_dv_next(dv, e, dv');
-        lem_inv_current_att_duty_is_either_none_or_latest_served_duty_dv_next(dv, e, dv');
-        lem_inv_available_current_att_duty_is_latest_served_att_duty_dv_next(dv, e, dv');        
-        lem_inv_is_sequence_attestation_duties_to_be_serves_orders_dv_next(dv, e, dv');                
+        lem_inv_none_latest_served_duty_implies_none_current_proposer_duty_dv_next(dv, e, dv');
+        lem_inv_current_proposer_duty_is_either_none_or_latest_served_duty_dv_next(dv, e, dv');
+        lem_inv_available_current_proposer_duty_is_latest_served_proposer_duty_dv_next(dv, e, dv');        
     }
 
-    lemma lem_ind_inv_dv_next_invs_group_3(dv: DVState, e: DV.Event, dv': DVState)       
-    requires DV.NextEventPreCond(dv, e)
-    requires DV.NextEvent(dv, e, dv')  
+    lemma lem_ind_inv_dv_next_invs_group_3(dv: DVState, e: DV_Block_Proposer_Spec.Event, dv': DVState)       
+    requires DV_Block_Proposer_Spec.NextEventPreCond(dv, e)
+    requires DV_Block_Proposer_Spec.NextEvent(dv, e, dv')  
     requires ind_inv(dv)
     ensures invs_group_3(dv')
     {
-        lem_inv_no_duplicated_att_duties_dv_next(dv, e, dv');
-        lem_inv_every_att_duty_before_dvn_att_index_was_delivered_dv_next(dv, e, dv');        
-        lem_inv_no_active_consensus_instance_before_receiving_an_att_duty_dv_next(dv, e, dv');                        
+        lem_inv_no_duplicated_proposer_duties_dv_next(dv, e, dv');
+        lem_inv_every_proposer_duty_before_dvn_proposer_index_was_delivered_dv_next(dv, e, dv');        
+        lem_inv_no_active_consensus_instance_before_receiving_a_proposer_duty_dv_next(dv, e, dv');                        
     }
 
-    lemma lem_ind_inv_dv_next_invs_group_4(dv: DVState, e: DV.Event, dv': DVState)       
-    requires DV.NextEventPreCond(dv, e)
-    requires DV.NextEvent(dv, e, dv')  
+    lemma lem_ind_inv_dv_next_invs_group_4(dv: DVState, e: DV_Block_Proposer_Spec.Event, dv': DVState)       
+    requires DV_Block_Proposer_Spec.NextEventPreCond(dv, e)
+    requires DV_Block_Proposer_Spec.NextEvent(dv, e, dv')  
     requires ind_inv(dv)
     ensures invs_group_4(dv')
     {
-        lem_inv_att_duty_in_next_delivery_is_not_lower_than_rcvd_att_duties_ind_inv(dv);
-        lem_inv_slot_of_active_consensus_instance_is_not_higher_than_slot_of_latest_served_att_duty_dv_next(dv, e, dv');                
-        lem_inv_consensus_instance_only_for_slot_in_which_dvc_has_rcvd_att_duty_dv_next(dv, e, dv');    
+        lem_inv_slot_of_active_consensus_instance_is_not_higher_than_slot_of_latest_served_proposer_duty_dv_next(dv, e, dv');                
+        lem_inv_consensus_instance_only_for_slot_in_which_dvc_has_rcvd_proposer_duty_dv_next(dv, e, dv');    
         lem_inv_consensus_instances_only_for_rcvd_duties_dv_next(dv, e, dv');    
-        lem_inv_rcvd_att_duty_is_from_dv_seq_for_rcvd_att_duty_dv_next(dv, e, dv');    
+        lem_inv_rcvd_proposer_duty_is_from_dv_seq_for_rcvd_proposer_duty_dv_next(dv, e, dv');    
     }
 
-    lemma lem_ind_inv_dv_next_invs_group_5(dv: DVState, e: DV.Event, dv': DVState)       
-    requires DV.NextEventPreCond(dv, e)
-    requires DV.NextEvent(dv, e, dv')  
+    lemma lem_ind_inv_dv_next_invs_group_5(dv: DVState, e: DV_Block_Proposer_Spec.Event, dv': DVState)       
+    requires DV_Block_Proposer_Spec.NextEventPreCond(dv, e)
+    requires DV_Block_Proposer_Spec.NextEvent(dv, e, dv')  
     requires ind_inv(dv)
     ensures invs_group_5(dv')
     {
-        lem_inv_att_slashing_db_hist_keeps_track_of_only_rcvd_att_duties_dv_next(dv, e, dv');    
-        lem_inv_exists_db_in_att_slashing_db_hist_and_duty_for_every_validity_predicate_dv_next(dv, e, dv');  
-        lem_inv_current_validity_predicate_for_slot_k_is_stored_in_att_slashing_db_hist_k_dv_next(dv, e, dv');          
+        lem_inv_block_slashing_db_hist_keeps_track_of_only_rcvd_proposer_duties_dv_next(dv, e, dv');    
+        lem_inv_exists_db_in_block_slashing_db_hist_and_proposer_duty_and_randao_reveal_for_every_validity_predicate_dv_next(dv, e, dv');  
+        lem_inv_current_validity_predicate_for_slot_k_is_stored_in_block_slashing_db_hist_k_dv_next(dv, e, dv');          
     }
 
-    lemma lem_ind_inv_dv_next_invs_group_6(dv: DVState, e: DV.Event, dv': DVState)       
-    requires DV.NextEventPreCond(dv, e)
-    requires DV.NextEvent(dv, e, dv')  
+    lemma lem_ind_inv_dv_next_invs_group_6(dv: DVState, e: DV_Block_Proposer_Spec.Event, dv': DVState)       
+    requires DV_Block_Proposer_Spec.NextEventPreCond(dv, e)
+    requires DV_Block_Proposer_Spec.NextEvent(dv, e, dv')  
     requires ind_inv(dv)
     ensures invs_group_6(dv')
     {       
-        lem_inv_every_db_in_att_slashing_db_hist_is_subset_of_att_slashing_db_dv_next(dv, e, dv');  
-        lem_inv_active_attn_consensus_instances_are_tracked_in_att_slashing_db_hist_dv_next(dv, e, dv');  
-        lem_inv_construct_signed_attestation_signature_assumptions_helper_dv_next(dv, e, dv');  
+        lem_inv_every_db_in_block_slashing_db_hist_is_subset_of_block_slashing_db_dv_next(dv, e, dv');  
+        lem_inv_active_consensus_instances_on_beacon_blocks_are_tracked_in_block_slashing_db_hist_dv_next(dv, e, dv');  
     }
 
-    lemma lem_ind_inv_dv_next_invs_group_7(dv: DVState, e: DV.Event, dv': DVState)       
-    requires DV.NextEventPreCond(dv, e)
-    requires DV.NextEvent(dv, e, dv')  
+    lemma lem_ind_inv_dv_next_invs_group_7(dv: DVState, e: DV_Block_Proposer_Spec.Event, dv': DVState)       
+    requires DV_Block_Proposer_Spec.NextEventPreCond(dv, e)
+    requires DV_Block_Proposer_Spec.NextEvent(dv, e, dv')  
     requires ind_inv(dv)
     ensures invs_group_7(dv')
     {               
         lem_inv_all_in_transit_messages_were_sent_dv_next(dv, e, dv');  
-        lem_inv_rcvd_attn_shares_are_from_sent_messages_dv_next(dv, e, dv');  
-        Invs_DV_Next_5.lem_inv_33(dv, e, dv');
+        lem_inv_rcvd_block_shares_are_from_sent_messages_dv_next(dv, e, dv');  
+        lem_inv_slots_for_sent_validity_predicate_are_stored_in_block_slashing_db_hist(dv, e, dv');
     }
 
     lemma lem_ind_inv_implies_intermediate_steps_helper_1(dv: DVState)
     requires ind_inv(dv)
-    ensures inv_att_duty_in_next_delivery_is_not_lower_than_current_att_duty(dv)
-    ensures inv_att_duty_in_next_delivery_is_not_lower_than_latest_served_att_duty(dv)
-    ensures inv_att_duty_in_next_delivery_is_not_lower_than_rcvd_att_duties(dv)
+    ensures inv_proposer_duty_in_next_delivery_is_higher_than_latest_served_proposer_duty(dv)
+    ensures inv_proposer_duty_in_next_delivery_is_not_lower_than_rcvd_proposer_duties(dv)
     {    
-        lem_inv_att_duty_in_next_delivery_is_not_lower_than_current_att_duty_ind_inv(dv);
-        lem_inv_att_duty_in_next_delivery_is_not_lower_than_latest_served_att_duty_ind_inv(dv);
-        lem_inv_att_duty_in_next_delivery_is_not_lower_than_rcvd_att_duties_ind_inv(dv);
+        lem_inv_proposer_duty_in_next_delivery_is_higher_than_latest_served_proposer_duty_ind_inv(dv);
+        lem_inv_proposer_duty_in_next_delivery_is_not_lower_than_rcvd_proposer_duties_ind_inv(dv);
     }
 
     lemma lem_ind_inv_implies_intermediate_steps_helper_2(dv: DVState)
     requires ind_inv(dv)  
-    ensures inv_sent_vp_is_based_on_existing_slashing_db_and_rcvd_att_duty(dv)
-    ensures inv_active_consensus_instances_implied_the_delivery_of_att_duties(dv)   
-    ensures same_honest_nodes_in_dv_and_ci(dv)    
-    ensures construct_signed_attestation_signature_assumptions_helper(
-                dv.construct_signed_attestation_signature,
+    ensures inv_sent_vp_is_based_on_existing_slashing_db_and_rcvd_proposer_duty_and_randao_reveal(dv)
+    ensures inv_active_consensus_instances_implied_the_delivery_of_proposer_duties(dv)   
+    ensures inv_same_node_status_in_dv_and_ci(dv)    
+    ensures construct_complete_signed_block_assumptions_helper(
+                dv.construct_complete_signed_block,
                 dv.dv_pubkey,
-                dv.all_nodes)  
+                dv.all_nodes
+            )  
     {    
-        lem_inv_sent_vp_is_based_on_existing_slashing_db_and_rcvd_att_duty_ind_inv(dv);
-        lem_inv_active_consensus_instances_implied_the_delivery_of_att_duties_ind_inv(dv);
-        lem_inv_queued_att_duty_is_rcvd_duty3_ind_inv(dv);      
-        lem_construct_signed_attestation_signature_assumptions_helper(dv);       
+        lem_inv_sent_vp_is_based_on_existing_slashing_db_and_rcvd_proposer_duty_and_randao_reveal_ind_inv(dv);
+        lem_inv_active_consensus_instances_implied_the_delivery_of_proposer_duties_ind_inv(dv);
+        lem_inv_same_node_status_in_dv_and_ci_ind_inv(dv);      
+        lem_construct_complete_signed_block_assumptions_helper(dv);       
     }
 
     lemma lem_ind_inv_implies_intermediate_steps_helper_3(dv: DVState)
     requires ind_inv(dv)  
-    ensures inv_sequence_attestation_duties_to_be_served_ordered(dv)
-    ensures inv_active_attestation_consensus_instances_keys_is_subset_of_att_slashing_db_hist(dv)
-    ensures inv_current_latest_attestation_duty_match(dv)
-    ensures inv_rcvd_attestation_shares_is_in_all_messages_sent(dv)
-    {    
-        lem_inv_active_attestation_consensus_instances_keys_is_subset_of_att_slashing_db_hist(dv);
-        lem_inv_current_latest_attestation_duty_match(dv);
-        lem_inv_rcvd_attn_shares_are_from_sent_messages_inv_rcvd_attestation_shares_is_in_all_messages_sent(dv);
+    ensures inv_seq_of_proposer_duties_is_ordered(dv)
+    ensures inv_active_consensus_instances_on_beacon_blocks_are_tracked_in_block_slashing_db_hist(dv)
+    ensures inv_current_latest_proposer_duty_match(dv)
+    ensures inv_rcvd_block_shares_are_in_all_sent_messages(dv)
+    {            
+        lem_inv_current_latest_proposer_duty_match(dv);
+        lem_inv_rcvd_block_shares_are_from_sent_messages_inv_rcvd_block_shares_are_in_all_sent_messages(dv);
     }
 
     lemma lem_ind_inv_implies_intermediate_steps_helper_4(dv: DVState)
     requires ind_inv(dv)  
-    ensures lem_inv_exists_honest_dvc_that_sent_att_share_for_submitted_att_new_precond(dv)    
-    ensures inv_data_of_all_created_attestations_is_set_of_decided_values(dv)
+    ensures lem_inv_exists_honest_dvc_that_sent_block_share_for_submitted_block_new_precond(dv)    
+    ensures inv_block_of_all_created_blocks_is_set_of_decided_values(dv)
     {   
         lem_ind_inv_implies_intermediate_steps_helper_1(dv);
         lem_ind_inv_implies_intermediate_steps_helper_2(dv);
         lem_ind_inv_implies_intermediate_steps_helper_3(dv);   
-        lem_inv_data_of_all_created_attestations_is_set_of_decided_values_dv_next(dv);
+        lem_inv_block_of_all_created_blocks_is_set_of_decided_values_dv_next(dv);
     }
 
     lemma lem_ind_inv_implies_intermediate_steps(dv: DVState)
     requires ind_inv(dv)
-    ensures inv_att_duty_in_next_delivery_is_not_lower_than_current_att_duty(dv)
-    ensures inv_att_duty_in_next_delivery_is_not_lower_than_latest_served_att_duty(dv)
-    ensures inv_att_duty_in_next_delivery_is_not_lower_than_rcvd_att_duties(dv)
-    ensures inv_sent_vp_is_based_on_existing_slashing_db_and_rcvd_att_duty(dv)
-    ensures inv_active_consensus_instances_implied_the_delivery_of_att_duties(dv)   
-    ensures same_honest_nodes_in_dv_and_ci(dv)    
-    ensures construct_signed_attestation_signature_assumptions_helper(
-                dv.construct_signed_attestation_signature,
+    ensures inv_proposer_duty_in_next_delivery_is_higher_than_latest_served_proposer_duty(dv)
+    ensures inv_proposer_duty_in_next_delivery_is_not_lower_than_rcvd_proposer_duties(dv)
+    ensures inv_sent_vp_is_based_on_existing_slashing_db_and_rcvd_proposer_duty_and_randao_reveal(dv)
+    ensures inv_active_consensus_instances_implied_the_delivery_of_proposer_duties(dv)   
+    ensures inv_same_node_status_in_dv_and_ci(dv)    
+    ensures construct_complete_signed_block_assumptions_helper(
+                dv.construct_complete_signed_block,
                 dv.dv_pubkey,
-                dv.all_nodes)  
-    ensures inv_sequence_attestation_duties_to_be_served_ordered(dv)     
-    ensures inv_active_attestation_consensus_instances_keys_is_subset_of_att_slashing_db_hist(dv)
-    ensures inv_current_latest_attestation_duty_match(dv)
-    ensures inv_rcvd_attestation_shares_is_in_all_messages_sent(dv)
-    ensures lem_inv_exists_honest_dvc_that_sent_att_share_for_submitted_att_new_precond(dv)
-    ensures inv_data_of_all_created_attestations_is_set_of_decided_values(dv)
+                dv.all_nodes
+            )    
+    ensures inv_seq_of_proposer_duties_is_ordered(dv)     
+    ensures inv_active_consensus_instances_on_beacon_blocks_are_tracked_in_block_slashing_db_hist(dv)
+    ensures inv_current_latest_proposer_duty_match(dv)
+    ensures inv_rcvd_block_shares_are_in_all_sent_messages(dv)
+    ensures lem_inv_exists_honest_dvc_that_sent_block_share_for_submitted_block_new_precond(dv)
+    ensures inv_block_of_all_created_blocks_is_set_of_decided_values(dv)
     {   
         lem_ind_inv_implies_intermediate_steps_helper_1(dv); 
         lem_ind_inv_implies_intermediate_steps_helper_2(dv);
         lem_ind_inv_implies_intermediate_steps_helper_3(dv);
         lem_ind_inv_implies_intermediate_steps_helper_4(dv);
-        lem_inv_sent_vp_is_based_on_existing_slashing_db_and_rcvd_att_duty_ind_inv(dv);
-        lem_inv_data_of_all_created_attestations_is_set_of_decided_values_dv_next(dv);
+        lem_inv_sent_vp_is_based_on_existing_slashing_db_and_rcvd_proposer_duty_and_randao_reveal_ind_inv(dv);
+        lem_inv_block_of_all_created_blocks_is_set_of_decided_values_dv_next(dv);
     }
    
-    lemma lem_ind_inv_dv_next_inv_all_validity_predicates_are_stored_in_att_slashing_db_hist(dv: DVState, e: DV.Event, dv': DVState)  
-    requires DV.NextEventPreCond(dv, e)
-    requires DV.NextEvent(dv, e, dv')       
-    requires ind_inv(dv)
-    ensures inv_all_validity_predicates_are_stored_in_att_slashing_db_hist(dv')
-    {
-        lem_inv_current_validity_predicate_for_slot_k_is_stored_in_att_slashing_db_hist_k_inv_active_attestation_consensus_instances_predicate_is_in_att_slashing_db_hist(dv);
-        assert inv_active_attestation_consensus_instances_predicate_is_in_att_slashing_db_hist(dv);
+    // lemma lem_ind_inv_dv_next_inv_all_validity_predicates_are_stored_in_block_slashing_db_hist(dv: DVState, e: DV_Block_Proposer_Spec.Event, dv': DVState)  
+    // requires DV_Block_Proposer_Spec.NextEventPreCond(dv, e)
+    // requires DV_Block_Proposer_Spec.NextEvent(dv, e, dv')       
+    // requires ind_inv(dv)
+    // ensures inv_all_validity_predicates_are_stored_in_block_slashing_db_hist(dv')
+    // {
+    //     // lem_inv_current_validity_predicate_for_slot_k_is_stored_in_block_slashing_db_hist_k_inv_active_block_consensus_instances_predicate_is_in_block_slashing_db_hist(dv);
+    //     // assert inv_active_block_consensus_instances_predicate_is_in_block_slashing_db_hist(dv);
 
-        lem_inv_active_attestation_consensus_instances_keys_is_subset_of_att_slashing_db_hist(dv);
-        assert inv_active_attestation_consensus_instances_keys_is_subset_of_att_slashing_db_hist(dv);
+    //     // lem_inv_active_consensus_instances_on_beacon_blocks_are_tracked_in_block_slashing_db_hist(dv);
+    //     // assert inv_active_consensus_instances_on_beacon_blocks_are_tracked_in_block_slashing_db_hist(dv);
 
-        lem_ind_inv_implies_intermediate_steps(dv);
-        assert same_honest_nodes_in_dv_and_ci(dv);
+    //     // lem_ind_inv_implies_intermediate_steps(dv);
+    //     // assert inv_same_node_status_in_dv_and_ci(dv);
 
 
-        assert && inv_all_validity_predicates_are_stored_in_att_slashing_db_hist(dv)
-               && inv_quorum_constraints(dv)
-               && same_honest_nodes_in_dv_and_ci(dv)
-               && inv_only_dv_construct_signed_attestation_signature(dv)    
-               && inv_slots_for_sent_validity_predicate_are_stored_in_att_slashing_db_hist(dv)  
-               && inv_active_attestation_consensus_instances_keys_is_subset_of_att_slashing_db_hist(dv)
-               && inv_active_attestation_consensus_instances_predicate_is_in_att_slashing_db_hist(dv)
-               ;
+    //     // assert && inv_all_validity_predicates_are_stored_in_block_slashing_db_hist(dv)
+    //     //        && inv_quorum_constraints(dv)
+    //     //        && inv_same_node_status_in_dv_and_ci(dv)
+    //     //        && inv_only_dv_construct_complete_signing_functions(dv)    
+    //     //        && inv_slots_for_sent_validity_predicate_are_stored_in_block_slashing_db_hist(dv)  
+    //     //        && inv_active_consensus_instances_on_beacon_blocks_are_tracked_in_block_slashing_db_hist(dv)
+    //     //        && inv_active_block_consensus_instances_predicate_is_in_block_slashing_db_hist(dv)
+    //     //        ;
 
-        lem_inv_all_validity_predicates_are_stored_in_att_slashing_db_hist(dv, e, dv');    
-        assert inv_all_validity_predicates_are_stored_in_att_slashing_db_hist(dv');
-    }
+    //     lem_inv_all_validity_predicates_are_stored_in_block_slashing_db_hist_dv_next(dv, e, dv');    
+    //     assert inv_all_validity_predicates_are_stored_in_block_slashing_db_hist(dv');
+    // }
 
-    lemma lem_ind_inv_dv_next_inv_exists_honest_dvc_that_sent_att_share_for_submitted_att(dv: DVState, e: DV.Event, dv': DVState)       
-    requires DV.NextEventPreCond(dv, e)
-    requires DV.NextEvent(dv, e, dv')  
-    requires ind_inv(dv)
-    ensures inv_exists_honest_dvc_that_sent_att_share_for_submitted_att(dv')
-    {
-        lem_ind_inv_implies_intermediate_steps(dv);
-        assert construct_signed_attestation_signature_assumptions_helper(
-                dv.construct_signed_attestation_signature,
-                dv.dv_pubkey,
-                dv.all_nodes);
+    // lemma lem_ind_inv_dv_next_inv_exists_honest_dvc_that_sent_block_share_for_submitted_block(dv: DVState, e: DV_Block_Proposer_Spec.Event, dv': DVState)       
+    // requires DV_Block_Proposer_Spec.NextEventPreCond(dv, e)
+    // requires DV_Block_Proposer_Spec.NextEvent(dv, e, dv')  
+    // requires ind_inv(dv)
+    // ensures inv_exists_honest_dvc_that_sent_block_share_for_submitted_block(dv')
+    // {
+    //     // lem_ind_inv_implies_intermediate_steps(dv);
+    //     // assert construct_signed_block_signature_assumptions_helper(
+    //     //         dv.construct_signed_block_signature,
+    //     //         dv.dv_pubkey,
+    //     //         dv.all_nodes);
 
-        lem_inv_all_in_transit_messages_were_sent_invNetwork(dv);
-        assert invNetwork(dv);
+    //     // lem_inv_all_in_transit_messages_were_sent_invNetwork(dv);
+    //     // assert invNetwork(dv);
 
-        lem_inv_rcvd_attn_shares_are_from_sent_messages_inv_rcvd_attestation_shares_is_in_all_messages_sent(dv);
-        assert inv_rcvd_attestation_shares_is_in_all_messages_sent(dv);
+    //     // lem_inv_rcvd_block_shares_are_from_sent_messages_inv_rcvd_block_shares_are_in_all_sent_messages(dv);
+    //     // assert inv_rcvd_block_shares_are_in_all_sent_messages(dv);
 
-        assert  && DV.NextEvent(dv, e, dv')
-                && inv_exists_honest_dvc_that_sent_att_share_for_submitted_att(dv)
-                && construct_signed_attestation_signature_assumptions_helper(
-                    dv.construct_signed_attestation_signature,
-                    dv.dv_pubkey,
-                    dv.all_nodes
-                )
-                && inv_only_dv_construct_signed_attestation_signature(dv)  
-                && invNetwork(dv)
-                && inv_quorum_constraints(dv)
-                && inv_rcvd_attestation_shares_is_in_all_messages_sent(dv)
-                ;
+    //     // assert  && DV_Block_Proposer_Spec.NextEvent(dv, e, dv')
+    //     //         && inv_exists_honest_dvc_that_sent_block_share_for_submitted_block(dv)
+    //     //         && construct_signed_block_signature_assumptions_helper(
+    //     //             dv.construct_signed_block_signature,
+    //     //             dv.dv_pubkey,
+    //     //             dv.all_nodes
+    //     //         )
+    //     //         && inv_only_dv_construct_complete_signing_functions(dv)  
+    //     //         && invNetwork(dv)
+    //     //         && inv_quorum_constraints(dv)
+    //     //         && inv_rcvd_block_shares_are_in_all_sent_messages(dv)
+    //     //         ;
 
         
-        lem_inv_exists_honest_dvc_that_sent_att_share_for_submitted_att_dv_next(dv, e, dv');
-        assert inv_exists_honest_dvc_that_sent_att_share_for_submitted_att(dv');
-    }
+    //     lem_inv_exists_honest_dvc_that_sent_block_share_for_submitted_block_dv_next(dv, e, dv');
+    //     assert inv_exists_honest_dvc_that_sent_block_share_for_submitted_block(dv');
+    // }
 
-    lemma lem_ind_inv_dv_next_inv_decided_value_of_consensus_instance_is_decided_by_quorum(dv: DVState, e: DV.Event, dv': DVState)       
-    requires DV.NextEventPreCond(dv, e)
-    requires DV.NextEvent(dv, e, dv')  
-    requires ind_inv(dv)
-    ensures inv_decided_value_of_consensus_instance_is_decided_by_quorum(dv')
-    {
-        lem_inv_decided_value_of_consensus_instance_is_decided_by_quorum(dv, e, dv');
-    }
+    // lemma lem_ind_inv_dv_next_inv_decided_value_of_consensus_instance_is_decided_by_quorum(dv: DVState, e: DV_Block_Proposer_Spec.Event, dv': DVState)       
+    // requires DV_Block_Proposer_Spec.NextEventPreCond(dv, e)
+    // requires DV_Block_Proposer_Spec.NextEvent(dv, e, dv')  
+    // requires ind_inv(dv)
+    // ensures inv_decided_value_of_consensus_instance_is_decided_by_quorum(dv')
+    // {
+    //     lem_inv_decided_value_of_consensus_instance_is_decided_by_quorum_dv_next(dv, e, dv');
+    // }
 
-    lemma lem_ind_inv_dv_next_inv_sent_validity_predicate_is_based_on_rcvd_att_duty_and_slashing_db_for_dv(dv: DVState, e: DV.Event, dv': DVState)       
-    requires DV.NextEventPreCond(dv, e)
-    requires DV.NextEvent(dv, e, dv')  
-    requires ind_inv(dv)
-    ensures inv_sent_validity_predicate_is_based_on_rcvd_att_duty_and_slashing_db_for_dv(dv')
-    {
-        lem_inv_sent_validity_predicate_is_based_on_rcvd_att_duty_and_slashing_db_for_dv_next(dv, e, dv');
-    }
+    // lemma lem_ind_inv_dv_next_inv_sent_validity_predicate_is_based_on_rcvd_proposer_duty_and_slashing_db_and_randao_reveal_for_dv(dv: DVState, e: DV_Block_Proposer_Spec.Event, dv': DVState)       
+    // requires DV_Block_Proposer_Spec.NextEventPreCond(dv, e)
+    // requires DV_Block_Proposer_Spec.NextEvent(dv, e, dv')  
+    // requires ind_inv(dv)
+    // ensures inv_sent_validity_predicate_is_based_on_rcvd_proposer_duty_and_slashing_db_and_randao_reveal_for_dv(dv')
+    // {
+    //     lem_inv_sent_validity_predicate_is_based_on_rcvd_proposer_duty_and_slashing_db_and_randao_reveal_for_dv_dv_next(dv, e, dv');
+    // }
 
-    lemma lem_ind_inv_dv_next_inv_sent_validity_predicate_is_based_on_rcvd_att_duty_and_slashing_db(dv: DVState, e: DV.Event, dv': DVState)       
-    requires DV.NextEventPreCond(dv, e)
-    requires DV.NextEvent(dv, e, dv')  
-    requires ind_inv(dv)
-    ensures inv_sent_validity_predicate_is_based_on_rcvd_att_duty_and_slashing_db(dv')
-    {
-        lem_inv_sent_validity_predicate_is_based_on_rcvd_att_duty_and_slashing_db(dv, e, dv');
-    }
+    // lemma lem_ind_inv_dv_next_inv_sent_validity_predicate_is_based_on_rcvd_proposer_duty_and_slashing_db_and_randao_reveal(dv: DVState, e: DV_Block_Proposer_Spec.Event, dv': DVState)       
+    // requires DV_Block_Proposer_Spec.NextEventPreCond(dv, e)
+    // requires DV_Block_Proposer_Spec.NextEvent(dv, e, dv')  
+    // requires ind_inv(dv)
+    // ensures inv_sent_validity_predicate_is_based_on_rcvd_proposer_duty_and_slashing_db_and_randao_reveal(dv')
+    // {
+    //     lem_inv_sent_validity_predicate_is_based_on_rcvd_proposer_duty_and_slashing_db_and_randao_reveal(dv, e, dv');
+    // }
 
-    lemma lem_ind_inv_dv_next_inv_decided_value_of_consensus_instance_of_slot_k_is_for_slot_k(dv: DVState, e: DV.Event, dv': DVState)       
-    requires DV.NextEventPreCond(dv, e)
-    requires DV.NextEvent(dv, e, dv')  
-    requires ind_inv(dv)
-    ensures inv_decided_value_of_consensus_instance_of_slot_k_is_for_slot_k(dv')
-    {
-        lem_inv_decided_value_of_consensus_instance_of_slot_k_is_for_slot_k(dv, e, dv');
-    }
+    // lemma lem_ind_inv_dv_next_inv_decided_value_of_consensus_instance_of_slot_k_is_for_slot_k(dv: DVState, e: DV_Block_Proposer_Spec.Event, dv': DVState)       
+    // requires DV_Block_Proposer_Spec.NextEventPreCond(dv, e)
+    // requires DV_Block_Proposer_Spec.NextEvent(dv, e, dv')  
+    // requires ind_inv(dv)
+    // ensures inv_decided_value_of_consensus_instance_of_slot_k_is_for_slot_k(dv')
+    // {
+    //     lem_inv_decided_value_of_consensus_instance_of_slot_k_is_for_slot_k_dv_next(dv, e, dv');
+    // }
 
     
-    lemma lem_ind_inv_dv_next_invs_group_8(dv: DVState, e: DV.Event, dv': DVState)       
-    requires DV.NextEventPreCond(dv, e)
-    requires DV.NextEvent(dv, e, dv')  
+    lemma lem_ind_inv_dv_next_invs_group_8(dv: DVState, e: DV_Block_Proposer_Spec.Event, dv': DVState)       
+    requires DV_Block_Proposer_Spec.NextEventPreCond(dv, e)
+    requires DV_Block_Proposer_Spec.NextEvent(dv, e, dv')  
     requires ind_inv(dv)
     ensures invs_group_8(dv')
     {
-        lem_ind_inv_dv_next_inv_all_validity_predicates_are_stored_in_att_slashing_db_hist(dv, e, dv');  
-        lem_ind_inv_dv_next_inv_exists_honest_dvc_that_sent_att_share_for_submitted_att(dv, e, dv');             
-        lem_ind_inv_dv_next_inv_decided_value_of_consensus_instance_is_decided_by_quorum(dv, e, dv');       
-        lem_ind_inv_dv_next_inv_sent_validity_predicate_is_based_on_rcvd_att_duty_and_slashing_db_for_dv(dv, e, dv');  
-        lem_ind_inv_dv_next_inv_sent_validity_predicate_is_based_on_rcvd_att_duty_and_slashing_db(dv, e, dv');   
+        lem_inv_exists_honest_dvc_that_sent_block_share_for_submitted_block_dv_next(dv, e, dv');
+        lem_inv_decided_value_of_consensus_instance_is_decided_by_quorum_dv_next(dv, e, dv');  
+        lem_inv_sent_validity_predicate_is_based_on_rcvd_proposer_duty_and_slashing_db_and_randao_reveal_for_dv_dv_next(dv, e, dv');
+        lem_inv_sent_validity_predicate_is_based_on_rcvd_proposer_duty_and_slashing_db_and_randao_reveal_dv_next(dv, e, dv');
+        // lem_ind_inv_dv_next_inv_all_validity_predicates_are_stored_in_block_slashing_db_hist(dv, e, dv');  
+        // lem_ind_inv_dv_next_inv_exists_honest_dvc_that_sent_block_share_for_submitted_block(dv, e, dv');             
+        // lem_ind_inv_dv_next_inv_decided_value_of_consensus_instance_is_decided_by_quorum(dv, e, dv');       
+        // lem_ind_inv_dv_next_inv_sent_validity_predicate_is_based_on_rcvd_proposer_duty_and_slashing_db_and_randao_reveal_for_dv(dv, e, dv');  
+        // lem_ind_inv_dv_next_inv_sent_validity_predicate_is_based_on_rcvd_proposer_duty_and_slashing_db_and_randao_reveal(dv, e, dv');   
     }
 
-    lemma lem_ind_inv_dv_next_invNetwork(dv: DVState, e: DV.Event, dv': DVState)       
-    requires DV.NextEventPreCond(dv, e)
-    requires DV.NextEvent(dv, e, dv')  
-    requires ind_inv(dv)
-    ensures invNetwork(dv')
-    {
-        lem_inv_all_in_transit_messages_were_sent_dv_next(dv, e, dv');
-        lem_inv_all_in_transit_messages_were_sent_invNetwork(dv');
-    }
+    // lemma lem_ind_inv_dv_next_invNetwork(dv: DVState, e: DV_Block_Proposer_Spec.Event, dv': DVState)       
+    // requires DV_Block_Proposer_Spec.NextEventPreCond(dv, e)
+    // requires DV_Block_Proposer_Spec.NextEvent(dv, e, dv')  
+    // requires ind_inv(dv)
+    // ensures invNetwork(dv')
+    // {
+    //     lem_inv_all_in_transit_messages_were_sent_dv_next(dv, e, dv');
+    //     lem_inv_all_in_transit_messages_were_sent_invNetwork(dv');
+    // }
 
-    lemma lem_ind_inv_dv_next_inv_38(dv: DVState, e: DV.Event, dv': DVState)       
-    requires DV.NextEventPreCond(dv, e)
-    requires DV.NextEvent(dv, e, dv')  
-    requires ind_inv(dv)
-    ensures inv_attestation_shares_to_broadcast_are_sent_messages(dv')
-    {
-        lem_ind_inv_implies_intermediate_steps(dv);
-        assert same_honest_nodes_in_dv_and_ci(dv);
-        lem_inv_attestation_shares_to_broadcast_are_sent_messages_dv_next(dv, e, dv');
-    }
+    // lemma lem_ind_inv_dv_next_inv_38(dv: DVState, e: DV_Block_Proposer_Spec.Event, dv': DVState)       
+    // requires DV_Block_Proposer_Spec.NextEventPreCond(dv, e)
+    // requires DV_Block_Proposer_Spec.NextEvent(dv, e, dv')  
+    // requires ind_inv(dv)
+    // ensures inv_block_shares_to_broadcast_are_sent_messages(dv')
+    // {
+    //     lem_ind_inv_implies_intermediate_steps(dv);
+    //     assert inv_same_node_status_in_dv_and_ci(dv);
+    //     lem_inv_block_shares_to_broadcast_are_sent_messages_dv_next(dv, e, dv');
+    // }
 
-    lemma lem_ind_inv_dv_next_inv_exists_att_duty_in_dv_seq_of_att_duty_for_every_slot_in_att_slashing_db_hist(dv: DVState, e: DV.Event, dv': DVState)       
-    requires DV.NextEventPreCond(dv, e)
-    requires DV.NextEvent(dv, e, dv')  
-    requires ind_inv(dv)
-    ensures inv_exists_att_duty_in_dv_seq_of_att_duty_for_every_slot_in_att_slashing_db_hist(dv')
-    {
-        lem_inv_exists_att_duty_in_dv_seq_of_att_duty_for_every_slot_in_att_slashing_db_hist(dv, e, dv');
-    }
+    // lemma lem_ind_inv_dv_next_inv_exists_proposer_duty_in_dv_seq_of_proposer_duties_for_every_slot_in_block_slashing_db_hist(dv: DVState, e: DV_Block_Proposer_Spec.Event, dv': DVState)       
+    // requires DV_Block_Proposer_Spec.NextEventPreCond(dv, e)
+    // requires DV_Block_Proposer_Spec.NextEvent(dv, e, dv')  
+    // requires ind_inv(dv)
+    // ensures inv_exists_proposer_duty_in_dv_seq_of_proposer_duties_for_every_slot_in_block_slashing_db_hist(dv')
+    // {
+    //     lem_inv_exists_proposer_duty_in_dv_seq_of_proposer_duties_for_every_slot_in_block_slashing_db_hist(dv, e, dv');
+    // }
 
-    lemma lem_ind_inv_dv_next_invs_group_9(dv: DVState, e: DV.Event, dv': DVState)       
-    requires DV.NextEventPreCond(dv, e)
-    requires DV.NextEvent(dv, e, dv')  
+    lemma lem_ind_inv_dv_next_invs_group_9(dv: DVState, e: DV_Block_Proposer_Spec.Event, dv': DVState)       
+    requires DV_Block_Proposer_Spec.NextEventPreCond(dv, e)
+    requires DV_Block_Proposer_Spec.NextEvent(dv, e, dv')  
     requires ind_inv(dv)
     ensures invs_group_9(dv')
     {
-        lem_inv_decided_value_of_consensus_instance_of_slot_k_is_for_slot_k(dv, e, dv');
-        lem_ind_inv_dv_next_invNetwork(dv, e, dv');
-        lem_ind_inv_dv_next_inv_38(dv, e, dv');
-        lem_inv_attestation_shares_to_broadcast_are_sent_messages_inv_attestation_shares_to_broadcast_is_a_subset_of_all_messages_sent(dv');
+        lem_inv_decided_value_of_consensus_instance_of_slot_k_is_for_slot_k_dv_next(dv, e, dv');
+        lem_inv_all_in_transit_messages_were_sent_dv_next(dv, e, dv');
+        lem_inv_all_in_transit_messages_were_sent_invNetwork(dv');
+        lem_inv_block_shares_to_broadcast_are_sent_messages_dv_next(dv, e, dv');        
     }
 
-    lemma lem_ind_inv_dv_next_invs_group_10(dv: DVState, e: DV.Event, dv': DVState)       
-    requires DV.NextEventPreCond(dv, e)
-    requires DV.NextEvent(dv, e, dv')  
+    lemma lem_ind_inv_dv_next_invs_group_10(dv: DVState, e: DV_Block_Proposer_Spec.Event, dv': DVState)       
+    requires DV_Block_Proposer_Spec.NextEventPreCond(dv, e)
+    requires DV_Block_Proposer_Spec.NextEvent(dv, e, dv')  
     requires ind_inv(dv)
     ensures invs_group_10(dv')
     {        
-        lem_ind_inv_dv_next_inv_exists_att_duty_in_dv_seq_of_att_duty_for_every_slot_in_att_slashing_db_hist(dv, e, dv');
-        lem_inv_available_latest_attestation_duty_is_from_dv_seq_of_att_duties_new_body_dv_next(dv, e, dv');
-        lem_inv_exists_att_duty_in_dv_seq_of_att_duty_for_every_slot_in_att_slashing_db_hist_a(dv, e, dv');
-        lem_ind_inv_implies_intermediate_steps(dv);
-        lem_inv_data_of_att_share_is_decided_value_dv_next(dv, e, dv');
+        lem_inv_available_latest_proposer_duty_is_from_dv_seq_of_proposer_duties_dv_next(dv, e, dv');
+        lem_ind_inv_implies_intermediate_steps(dv);        
+        lem_inv_available_current_proposer_duty_is_from_dv_seq_of_proposer_duties_dv_next(dv, e, dv');        
+        lem_inv_block_of_in_transit_block_share_is_decided_value_dv_next(dv, e, dv');
+        lem_inv_exists_proposer_duty_in_dv_seq_of_proposer_duties_for_every_slot_in_block_slashing_db_hist_dv_next(dv, e, dv');
     }
     
-    lemma lem_ind_inv_dv_next_inv_future_decided_data_of_dvc_is_consistent_with_existing_decision_dv(dv: DVState, e: DV.Event, dv': DVState)       
-    requires DV.NextEventPreCond(dv, e)
-    requires DV.NextEvent(dv, e, dv')  
-    requires ind_inv(dv)
-    ensures inv_future_decided_data_of_dvc_is_consistent_with_existing_decision_dv(dv')
-    {
-        lem_ind_inv_implies_intermediate_steps_helper_4(dv);
-        assert lem_inv_exists_honest_dvc_that_sent_att_share_for_submitted_att_new_precond(dv);
-        lem_inv_future_decided_data_of_dvc_is_consistent_with_existing_decision_dv(dv, e, dv');
-    }
+    // lemma lem_ind_inv_dv_next_inv_future_decided_data_of_dvc_is_consistent_with_existing_decision_dv(dv: DVState, e: DV_Block_Proposer_Spec.Event, dv': DVState)       
+    // requires DV_Block_Proposer_Spec.NextEventPreCond(dv, e)
+    // requires DV_Block_Proposer_Spec.NextEvent(dv, e, dv')  
+    // requires ind_inv(dv)
+    // ensures inv_future_decided_data_of_dvc_is_consistent_with_existing_decision_dv(dv')
+    // {
+    //     lem_ind_inv_implies_intermediate_steps_helper_4(dv);
+    //     assert lem_inv_exists_honest_dvc_that_sent_block_share_for_submitted_block_new_precond(dv);
+    //     lem_inv_future_decided_data_of_dvc_is_consistent_with_existing_decision_dv(dv, e, dv');
+    // }
 
-    lemma lem_ind_inv_dv_next_inv_slot_in_future_decided_data_is_correct(dv: DVState, e: DV.Event, dv': DVState)       
-    requires DV.NextEventPreCond(dv, e)
-    requires DV.NextEvent(dv, e, dv')  
-    requires ind_inv(dv)
-    ensures inv_slot_in_future_decided_data_is_correct(dv')
-    {
-        lem_ind_inv_implies_intermediate_steps_helper_4(dv);
-        lem_inv_slot_in_future_decided_data_is_correct(dv, e, dv');
-    }
+    // lemma lem_ind_inv_dv_next_inv_slot_in_future_beacon_block_is_correct(dv: DVState, e: DV_Block_Proposer_Spec.Event, dv': DVState)       
+    // requires DV_Block_Proposer_Spec.NextEventPreCond(dv, e)
+    // requires DV_Block_Proposer_Spec.NextEvent(dv, e, dv')  
+    // requires ind_inv(dv)
+    // ensures inv_slot_in_future_beacon_block_is_correct(dv')
+    // {
+    //     lem_ind_inv_implies_intermediate_steps_helper_4(dv);
+    //     lem_inv_slot_in_future_beacon_block_is_correct_dv_next(dv, e, dv');
+    // }
 
-    lemma lem_ind_inv_dv_next_invs_group_11(dv: DVState, e: DV.Event, dv': DVState)       
-    requires DV.NextEventPreCond(dv, e)
-    requires DV.NextEvent(dv, e, dv')  
+    lemma lem_ind_inv_dv_next_invs_group_11(dv: DVState, e: DV_Block_Proposer_Spec.Event, dv': DVState)       
+    requires DV_Block_Proposer_Spec.NextEventPreCond(dv, e)
+    requires DV_Block_Proposer_Spec.NextEvent(dv, e, dv')  
     requires ind_inv(dv)
     ensures invs_group_11(dv')
     {
         lem_ind_inv_implies_intermediate_steps_helper_4(dv);
         lem_inv_future_decided_data_of_dvc_is_consistent_with_existing_decision_dv(dv, e, dv');
-        lem_inv_slot_in_future_decided_data_is_correct(dv, e, dv');        
+        lem_inv_slot_in_future_beacon_block_is_correct_dv_next(dv, e, dv');    
+        lem_inv_none_latest_proposer_duty_and_empty_set_of_rcvd_proposer_duties_dv_next(dv, e, dv');   
+        lem_inv_unique_rcvd_proposer_duty_per_slot_dv_next(dv, e, dv');     
     }
 
-    lemma lem_ind_inv_dv_next_invs_group_12(dv: DVState, e: DV.Event, dv': DVState)       
-    requires DV.NextEventPreCond(dv, e)
-    requires DV.NextEvent(dv, e, dv')  
+    lemma lem_ind_inv_dv_next_invs_group_12(dv: DVState, e: DV_Block_Proposer_Spec.Event, dv': DVState)       
+    requires DV_Block_Proposer_Spec.NextEventPreCond(dv, e)
+    requires DV_Block_Proposer_Spec.NextEvent(dv, e, dv')  
     requires ind_inv(dv)
     ensures invs_group_12(dv')
     {
         lem_ind_inv_implies_intermediate_steps_helper_4(dv);
-        lem_inv_sent_validity_predicate_only_for_slots_stored_in_att_slashing_db_hist(dv, e, dv');
-        lem_inv_all_validity_predicates_are_stored_in_att_slashing_db_hist(dv, e, dv');
-        lem_inv_consensus_instances_are_isConditionForSafetyTrue_dv_next(dv, e, dv');  
-        lem_inv_unique_rcvd_att_duty_per_slot_dv_next(dv, e, dv');  
-        lem_inv_none_latest_att_duty_and_empty_set_of_rcvd_att_duties_dv_next(dv, e, dv');  
-        lem_inv_no_rcvd_att_duty_is_higher_than_latest_att_duty_dv_next(dv, e, dv');  
+        lem_inv_consensus_instance_isConditionForSafetyTrue_dv_next(dv, e, dv');   
+        lem_inv_no_rcvd_proposer_duty_is_higher_than_latest_proposer_duty_dv_next(dv, e, dv');  
+        lem_inv_sent_validity_predicate_only_for_slots_stored_in_block_slashing_db_hist(dv, e, dv');
+        lem_inv_all_validity_predicates_are_stored_in_block_slashing_db_hist_dv_next(dv, e, dv');
     }
 
-    lemma lem_ind_inv_dv_next_invs_group_13(dv: DVState, e: DV.Event, dv': DVState)       
-    requires DV.NextEventPreCond(dv, e)
-    requires DV.NextEvent(dv, e, dv')  
+    lemma lem_ind_inv_dv_next_invs_group_13(dv: DVState, e: DV_Block_Proposer_Spec.Event, dv': DVState)       
+    requires DV_Block_Proposer_Spec.NextEventPreCond(dv, e)
+    requires DV_Block_Proposer_Spec.NextEvent(dv, e, dv')  
     requires ind_inv(dv)
     ensures invs_group_13(dv')
     {
-        lem_inv_decided_data_has_an_honest_witness_dv_next(dv, e, dv');
-        lem_inv_all_created_attestations_are_valid_dv_next(dv, e, dv');
-        lem_inv_attestation_is_created_with_shares_from_quorum_dv_next(dv, e, dv');
         lem_inv_unchanged_dvc_rs_pubkey_dv_next(dv, e, dv');
+        lem_inv_all_created_signed_beacon_blocks_are_valid_dv_next(dv, e, dv');
+        lem_inv_complete_block_is_created_with_shares_from_quorum_dv_next(dv, e, dv');
+        lem_inv_exists_an_honest_dvc_as_a_witness_for_every_decided_beacon_block_dv_next(dv, e, dv');
     }
 
-    lemma lem_ind_inv_dv_next_invs_group_14(dv: DVState, e: DV.Event, dv': DVState)       
-    requires DV.NextEventPreCond(dv, e)
-    requires DV.NextEvent(dv, e, dv')  
+    lemma lem_ind_inv_dv_next_invs_group_14(dv: DVState, e: DV_Block_Proposer_Spec.Event, dv': DVState)       
+    requires DV_Block_Proposer_Spec.NextEventPreCond(dv, e)
+    requires DV_Block_Proposer_Spec.NextEvent(dv, e, dv')  
     requires ind_inv(dv)
     ensures invs_group_14(dv')
     {   
+        lem_inv_seq_of_proposer_duties_is_ordered_dv_next(dv, e, dv');
+        lem_inv_block_shares_to_broadcast_is_tracked_in_block_slashing_db_dv_next(dv, e, dv');
+        lem_inv_block_of_block_shares_is_known_dv_next(dv, e, dv');
+        lem_inv_slot_of_consensus_instance_is_up_to_slot_of_latest_proposer_duty_dv_next(dv, e, dv');
+        lem_inv_db_of_vp_contains_all_beacon_block_of_sent_block_shares_for_lower_slots_dv_next(dv, e, dv');        
+    }
+
+    lemma lem_ind_inv_dv_next_invs_group_15(dv: DVState, e: DV_Block_Proposer_Spec.Event, dv': DVState)       
+    requires DV_Block_Proposer_Spec.NextEventPreCond(dv, e)
+    requires DV_Block_Proposer_Spec.NextEvent(dv, e, dv')  
+    requires ind_inv(dv)
+    ensures invs_group_15(dv')
+    {   
+        lem_inv_none_latest_proposer_duty_implies_emply_block_slashing_db_dv_next(dv, e, dv');
+        lem_inv_slots_in_slashing_db_is_not_higher_than_slot_of_latest_proposer_duty_dv_next(dv, e, dv');
         
-        lem_inv_sequence_attestation_duties_to_be_served_ordered_dv_next(dv, e, dv');
-        lem_inv_att_shares_to_broadcast_is_tracked_in_attestation_slashing_db_dv_next(dv, e, dv');
-        lem_inv_data_of_att_shares_is_known_dv_next(dv, e, dv');
-        lem_inv_slot_of_consensus_instance_is_up_to_slot_of_latest_attestation_duty(dv, e, dv');
-        lem_inv_active_attestation_consensus_instances_keys_is_subset_of_att_slashing_db_hist(dv);   
-        lem_inv_db_of_vp_contains_all_att_data_of_sent_att_shares_for_lower_slots_dv_next(dv, e, dv');        
+        lem_inv_exists_honest_dvc_that_sent_block_share_for_submitted_block_dv_next(dv, e, dv');
+        lem_inv_block_of_in_transit_block_share_is_decided_value_dv_next(dv, e, dv');
+        lem_inv_all_created_signed_beacon_blocks_are_valid_dv_next(dv, e, dv');
+        lem_inv_block_of_all_created_blocks_is_set_of_decided_values_dv_next(dv');
+        lem_inv_at_most_submitted_signed_beacon_block_for_every_slot_dv_next(dv');
     }
     
-    lemma lem_ind_inv_dv_next_ind_inv_helper_1(dv: DVState, e: DV.Event, dv': DVState)       
-    requires DV.NextEventPreCond(dv, e)
-    requires DV.NextEvent(dv, e, dv')  
+    lemma lem_ind_inv_dv_next_ind_inv_helper_1(dv: DVState, e: DV_Block_Proposer_Spec.Event, dv': DVState)       
+    requires DV_Block_Proposer_Spec.NextEventPreCond(dv, e)
+    requires DV_Block_Proposer_Spec.NextEvent(dv, e, dv')  
     requires ind_inv(dv)
     ensures invs_group_1(dv')
     ensures invs_group_2(dv')
@@ -457,9 +472,9 @@ module Ind_Inv_DV_Next
         lem_ind_inv_dv_next_invs_group_3(dv, e, dv');
     }
 
-    lemma lem_ind_inv_dv_next_ind_inv_helper_2(dv: DVState, e: DV.Event, dv': DVState)  
-    requires DV.NextEventPreCond(dv, e)
-    requires DV.NextEvent(dv, e, dv')  
+    lemma lem_ind_inv_dv_next_ind_inv_helper_2(dv: DVState, e: DV_Block_Proposer_Spec.Event, dv': DVState)  
+    requires DV_Block_Proposer_Spec.NextEventPreCond(dv, e)
+    requires DV_Block_Proposer_Spec.NextEvent(dv, e, dv')  
     requires ind_inv(dv)    
     ensures invs_group_4(dv')
     ensures invs_group_5(dv')
@@ -474,9 +489,9 @@ module Ind_Inv_DV_Next
         lem_ind_inv_dv_next_invs_group_8(dv, e, dv');
     }
 
-    lemma lem_ind_inv_dv_next_ind_inv_helper_3(dv: DVState, e: DV.Event, dv': DVState)       
-    requires DV.NextEventPreCond(dv, e)
-    requires DV.NextEvent(dv, e, dv')  
+    lemma lem_ind_inv_dv_next_ind_inv_helper_3(dv: DVState, e: DV_Block_Proposer_Spec.Event, dv': DVState)       
+    requires DV_Block_Proposer_Spec.NextEventPreCond(dv, e)
+    requires DV_Block_Proposer_Spec.NextEvent(dv, e, dv')  
     requires ind_inv(dv)
     ensures invs_group_9(dv')
     ensures invs_group_10(dv')
@@ -487,22 +502,31 @@ module Ind_Inv_DV_Next
         lem_ind_inv_dv_next_invs_group_11(dv, e, dv');                                     
     }
 
-    lemma lem_ind_inv_dv_next_ind_inv_helper_4(dv: DVState, e: DV.Event, dv': DVState)       
-    requires DV.NextEventPreCond(dv, e)
-    requires DV.NextEvent(dv, e, dv')  
+    lemma lem_ind_inv_dv_next_ind_inv_helper_4(dv: DVState, e: DV_Block_Proposer_Spec.Event, dv': DVState)       
+    requires DV_Block_Proposer_Spec.NextEventPreCond(dv, e)
+    requires DV_Block_Proposer_Spec.NextEvent(dv, e, dv')  
     requires ind_inv(dv)
     ensures invs_group_12(dv')   
-    ensures invs_group_13(dv')    
-    ensures invs_group_14(dv')
+    ensures invs_group_13(dv')            
     {        
         lem_ind_inv_dv_next_invs_group_12(dv, e, dv');                              
-        lem_ind_inv_dv_next_invs_group_13(dv, e, dv');     
-        lem_ind_inv_dv_next_invs_group_14(dv, e, dv');                              
+        lem_ind_inv_dv_next_invs_group_13(dv, e, dv');             
     }
 
-    lemma lem_ind_inv_dv_next_ind_inv_helper_a(dv: DVState, e: DV.Event, dv': DVState)       
-    requires DV.NextEventPreCond(dv, e)
-    requires DV.NextEvent(dv, e, dv')  
+    lemma lem_ind_inv_dv_next_ind_inv_helper_5(dv: DVState, e: DV_Block_Proposer_Spec.Event, dv': DVState)       
+    requires DV_Block_Proposer_Spec.NextEventPreCond(dv, e)
+    requires DV_Block_Proposer_Spec.NextEvent(dv, e, dv')  
+    requires ind_inv(dv)    
+    ensures invs_group_14(dv')
+    ensures invs_group_15(dv')
+    {        
+        lem_ind_inv_dv_next_invs_group_14(dv, e, dv');                              
+        lem_ind_inv_dv_next_invs_group_15(dv, e, dv');                              
+    }
+
+    lemma lem_ind_inv_dv_next_ind_inv_helper_a(dv: DVState, e: DV_Block_Proposer_Spec.Event, dv': DVState)       
+    requires DV_Block_Proposer_Spec.NextEventPreCond(dv, e)
+    requires DV_Block_Proposer_Spec.NextEvent(dv, e, dv')  
     requires ind_inv(dv) 
     ensures invs_group_1(dv')
     ensures invs_group_2(dv')
@@ -517,9 +541,9 @@ module Ind_Inv_DV_Next
         lem_ind_inv_dv_next_ind_inv_helper_2(dv, e, dv');    
     }
 
-    lemma lem_ind_inv_dv_next_ind_inv_helper_b(dv: DVState, e: DV.Event, dv': DVState)       
-    requires DV.NextEventPreCond(dv, e)
-    requires DV.NextEvent(dv, e, dv')  
+    lemma lem_ind_inv_dv_next_ind_inv_helper_b(dv: DVState, e: DV_Block_Proposer_Spec.Event, dv': DVState)       
+    requires DV_Block_Proposer_Spec.NextEventPreCond(dv, e)
+    requires DV_Block_Proposer_Spec.NextEvent(dv, e, dv')  
     requires ind_inv(dv) 
     ensures invs_group_9(dv')    
     ensures invs_group_10(dv')    
@@ -527,14 +551,16 @@ module Ind_Inv_DV_Next
     ensures invs_group_12(dv')    
     ensures invs_group_13(dv')    
     ensures invs_group_14(dv')
+    ensures invs_group_15(dv')
     {
         lem_ind_inv_dv_next_ind_inv_helper_3(dv, e, dv');   
         lem_ind_inv_dv_next_ind_inv_helper_4(dv, e, dv');    
+        lem_ind_inv_dv_next_ind_inv_helper_5(dv, e, dv');    
     }
 
-    lemma lem_ind_inv_dv_next_ind_inv_helper(dv: DVState, e: DV.Event, dv': DVState)       
-    requires DV.NextEventPreCond(dv, e)
-    requires DV.NextEvent(dv, e, dv')  
+    lemma lem_ind_inv_dv_next_ind_inv_helper(dv: DVState, e: DV_Block_Proposer_Spec.Event, dv': DVState)       
+    requires DV_Block_Proposer_Spec.NextEventPreCond(dv, e)
+    requires DV_Block_Proposer_Spec.NextEvent(dv, e, dv')  
     requires ind_inv(dv) 
     ensures invs_group_1(dv')
     ensures invs_group_2(dv')   
@@ -550,14 +576,15 @@ module Ind_Inv_DV_Next
     ensures invs_group_12(dv')    
     ensures invs_group_13(dv')    
     ensures invs_group_14(dv')    
+    ensures invs_group_15(dv')    
     {   
         lem_ind_inv_dv_next_ind_inv_helper_a(dv, e, dv');
         lem_ind_inv_dv_next_ind_inv_helper_b(dv, e, dv');                
     }
 
-    lemma lem_ind_inv_dv_next_ind_inv(dv: DVState, e: DV.Event, dv': DVState)       
-    requires DV.NextEventPreCond(dv, e)
-    requires DV.NextEvent(dv, e, dv')  
+    lemma lem_ind_inv_dv_next_ind_inv(dv: DVState, e: DV_Block_Proposer_Spec.Event, dv': DVState)       
+    requires DV_Block_Proposer_Spec.NextEventPreCond(dv, e)
+    requires DV_Block_Proposer_Spec.NextEvent(dv, e, dv')  
     requires ind_inv(dv)    
     ensures ind_inv(dv')    
     {   
@@ -565,11 +592,11 @@ module Ind_Inv_DV_Next
     }
 
     lemma lem_ind_inv_dv_ind_inv_NextPreCond(dv: DVState, dv': DVState)       
-    requires DV.NextPreCond(dv)
-    requires DV.Next(dv, dv')  
+    requires DV_Block_Proposer_Spec.NextPreCond(dv)
+    requires DV_Block_Proposer_Spec.Next(dv, dv')  
     requires ind_inv(dv)    
     ensures ind_inv(dv')  
-    ensures DV.NextPreCond(dv')
+    ensures DV_Block_Proposer_Spec.NextPreCond(dv')
     {
         var e :|
             && validEvent(dv, e)
