src/proofs/no_slashable_blocks/supporting_lemmas/init_implies_ind_inv/init_implies_ind_inv.dfy
@@ -1,33 +1,38 @@
-include "../../../../common/commons.dfy"
-include "../../common/attestation_creation_instrumented.dfy"
-include "../../../../specs/consensus/consensus.dfy"
-include "../../../../specs/network/network.dfy"
-include "../../../../specs/dv/dv_attestation_creation.dfy"
+include "../../../../common/block_proposer/block_types.dfy"
+include "../../../../common/block_proposer/block_common_functions.dfy"
+include "../../../../common/block_proposer/block_signing_functions.dfy"
+include "../../common/dvc_block_proposer_instrumented.dfy"
+
+include "../../../../specs/consensus/block_consensus.dfy"
+include "../../../../specs/network/block_network.dfy"
+include "../../../../specs/dv/dv_block_proposer.dfy"
+
 include "../inv.dfy"
 include "../ind_inv.dfy"
 
 module Ind_Inv_DV_Init
 {
-    import opened Types 
-    import opened CommonFunctions
-    import opened ConsensusSpec
-    import opened NetworkSpec
-    import opened DVC_Spec
-    import opened DV
-    import opened Att_Ind_Inv_With_Empty_Init_Att_Slashing_DB
-    import opened Att_Inv_With_Empty_Initial_Attestation_Slashing_DB
+    import opened Block_Types
+    import opened Block_Signing_Functions
+    import opened Block_Common_Functions
+    import opened Block_Consensus_Spec
+    import opened Block_Network_Spec
+    import opened DVC_Block_Proposer_Spec_Instr
+    import opened DV_Block_Proposer_Spec 
+    import opened Block_Inv_With_Empty_Initial_Block_Slashing_DB
+    import opened Block_Ind_Inv_With_Empty_Initial_Block_Slashing_DB
     
     lemma lem_ind_inv_dv_init(dv: DVState)       
-    requires DV.Init(dv, {})    
+    requires DV_Block_Proposer_Spec.Init(dv, {})    
     ensures ind_inv(dv)
     ensures NextPreCond(dv)
     {
-        assert  DV.Init(dv, {})  
+        assert  DV_Block_Proposer_Spec.Init(dv, {})  
                 ==>                 
                 && invs_group_1(dv)
                 && invs_group_2(dv)
         ;
-        assert  DV.Init(dv, {})  
+        assert  DV_Block_Proposer_Spec.Init(dv, {})  
                 ==>                 
                 && invs_group_3(dv)                         
                 && invs_group_4(dv)
@@ -35,7 +40,7 @@ module Ind_Inv_DV_Init
                 && invs_group_6(dv)                     
         ;
 
-        assert  DV.Init(dv, {})    
+        assert  DV_Block_Proposer_Spec.Init(dv, {})    
                 ==>
                 && invs_group_7(dv)
                 && invs_group_8(dv)           
@@ -45,6 +50,7 @@ module Ind_Inv_DV_Init
                 && invs_group_12(dv)
                 && invs_group_13(dv)
                 && invs_group_14(dv)
+                && invs_group_15(dv)
         ;
     }  
 }
